New induction principle for pairs of session types
Sty_ind2 now works with what I've dubbed a syncprod, rather than the
symprod from the standard library. The latter intuitively has
(x, y) < (x', y') if either x < x' or y < y'. The former has
(x, y) < (x', y') if both x < x' and y < y'. This turns out to be more
practical when dealing with equivalence proofs because for example for
send constructors, we usually need to prove (send B S, send B' S') given
(S, S').

Sty_ind2 uses the syncprod of lt_Sty, i.e. the construction order where
S < S' iff S' can be constructed by applying a finite number of
constructors to S.

SessionTypesInd.v
@@ -1,6 +1,6 @@
 Require Import Arith.Wf_nat Relations.Relation_Operators
   Wellfounded.Lexicographic_Product.
-Require Import SessionTypes Tac Var.
+Require Import SessionTypes Tac Var Wellfounded_Syncprod.
 
 (*****************************************************************************)
 (* Construction order *)
@@ -29,12 +29,20 @@ Proof. red. induction a; constructor; introv H; inverts H; auto. Defined.
 
 
 Definition lt_Sty2 : Sty * Sty -> Sty * Sty -> Prop
-  := symprod Sty Sty lt_Sty lt_Sty.
+  := syncprod lt_Sty lt_Sty.
 
 
 Lemma lt_Sty2_wf : well_founded lt_Sty2.
-Proof. apply wf_symprod; apply lt_Sty_wf. Defined.
+Proof. apply wf_syncprod; apply lt_Sty_wf. Defined.
 
+
+Lemma Sty_ind2 :
+  forall (P : Sty -> Sty -> Prop),
+  (forall S S',
+    (forall T T', lt_Sty2 (T, T') (S, S') -> P T T') ->
+    P S S') ->
+  forall S S', P S S'.
+Proof. intro P. apply (well_founded_induction_type_2 P lt_Sty2_wf). Qed.
 
 (*****************************************************************************)
 (* Order by length of longest prefix consisting only of mu constructors *)
