Wellfounded_Syncprod.v
@@ -1,0 +1,22 @@
+Require Import Relations Wellfounded.
+Require Import Tac.
+
+Inductive syncprod {A B} (RA : A -> A -> Prop) (RB : B -> B -> Prop) :
+  (A * B) -> (A * B) -> Prop :=
+| syncprod_intro :
+    forall a a' b b',
+    RA a a' ->
+    RB b b' ->
+    syncprod RA RB (a, b) (a', b')
+.
+
+
+Lemma wf_syncprod :
+  forall (A B : Type) RA RB,
+  well_founded RA ->
+  well_founded (@syncprod A B RA RB).
+Proof.
+  introv HwfA. unfolds. intro p. destruct p as [x y]. gen x y.
+  induction x using (well_founded_ind HwfA). intros.
+  constructor. introv H'. inverts H'. auto.
+Defined.
